1. Previous version of semax_ram contains existential inside the definition. This does not work with extract_exists_pre. Current definition remove that part, but take good use of Coq's environment system. 2. Make progress in verif_mark.

floyd_ext/semax_ram_lemmas.v
@@ -1,35 +1,68 @@
+Require Import RamifyCoq.Coqlib.
 Require Import VST.floyd.base.
 Require Import VST.floyd.canon.
 Require Import VST.floyd.assert_lemmas.
 Require Import VST.floyd.client_lemmas.
-Require Import RamifyCoq.veric_ext.seplog.
-Require Import RamifyCoq.veric_ext.SeparationLogic.
 
 Local Open Scope logic.
+
+Module RAM_FRAME.
+
+Record SingleFrame' l g s: Type := {
+  frame: environ -> mpred;
+  frame_sound: g |-- l * frame;
+  frame_closed: Forall (fun s => closed_wrt_modvars s frame) s
+}.
+
+Record SingleFrame: Type := {
+  local_assert: environ -> mpred;
+  global_assert: environ -> mpred;
+  stats: list statement;
+  real_frame: SingleFrame' local_assert global_assert stats
+}.
+
+End RAM_FRAME.
+
+Definition SingleFrame' := RAM_FRAME.SingleFrame'.
+Definition SingleFrame := RAM_FRAME.SingleFrame.
+
+Arguments RAM_FRAME.Build_SingleFrame' {l} {g} {s} frame frame_sound frame_closed.
 
 Section SEMAX.
 
 Context {Espec: OracleKind}.
 
-Record SingleFrame: Type := {
-  local_assert: environ -> mpred;
-  global_assert: environ -> mpred;
-  stats: list statement
-}.
+Inductive add_stats (s0: statement) : list SingleFrame -> list SingleFrame -> Prop :=
+  | add_stats_nil : add_stats s0 nil nil
+  | add_stats_cons : forall l g s f fs fs' fc fc' F F', add_stats s0 F F' ->
+      add_stats s0
+       (RAM_FRAME.Build_SingleFrame l g s (RAM_FRAME.Build_SingleFrame' f fs fc) :: F)
+       (RAM_FRAME.Build_SingleFrame l g (s0 :: s) (RAM_FRAME.Build_SingleFrame' f fs' fc') :: F')
+  .
 
-Definition add_stat s0 (f: SingleFrame) :=
-  Build_SingleFrame (local_assert f) (global_assert f) (s0 :: (stats f)).
+Definition SingleFrame'_inv {l g s0 s} (F: SingleFrame' l g (s0 :: s)) : SingleFrame' l g s :=
+  match F with
+  | RAM_FRAME.Build_SingleFrame' f fs fc =>
+      RAM_FRAME.Build_SingleFrame' f fs (Coqlib.Forall_tl _ _ _ fc)
+  end.
 
-Definition add_stats s0 fs := map (add_stat s0) fs.
+Lemma eexists_add_stats_cons: forall s0 l g s (F0: SingleFrame' _ _ _) F F',
+  add_stats s0 F F' ->
+  add_stats s0
+   (RAM_FRAME.Build_SingleFrame l g s (SingleFrame'_inv F0) :: F)
+   (RAM_FRAME.Build_SingleFrame l g (s0 :: s) F0 :: F').
+Proof.
+  intros.
+  destruct F0; unfold SingleFrame'_inv.
+  constructor.
+  auto.
+Qed.
 
 Fixpoint semax_ram (Delta: tycontext) (F: list SingleFrame) (P: environ -> mpred) (c: statement) (Q: ret_assert): Prop :=
   match F with
   | nil => semax Delta P c Q
-  | Build_SingleFrame l g s :: F_tail =>
-      exists F0,
-        g |-- l * F0 /\
-        Forall (fun s => closed_wrt_modvars s F0) s /\
-        semax_ram Delta F_tail (P * F0) c Q
+  | RAM_FRAME.Build_SingleFrame _ _ _ (RAM_FRAME.Build_SingleFrame' F0 _ _) :: F_tail =>
+      semax_ram Delta F_tail (P * F0) c Q
   end.
 
 Lemma semax_ram_pre: forall Delta F P P' c Q,
@@ -42,68 +75,95 @@ Opaque LiftNatDed' LiftSepLog'.
   revert P P' H0 H; induction F; intros; simpl in H0 |- *.
 Transparent LiftNatDed' LiftSepLog'.
   + eapply semax_pre0; eauto.
-  + destruct a as [l g s].
-    destruct H0 as [F0 [? [? ?]]].
-    exists F0.
-    split; [| split]; auto. 
+  + destruct a as [l g s [F0 ? ?]].
     eapply IHF; eauto.
     apply sepcon_derives; auto.
 Qed.
 
 Lemma semax_ram_localize: forall Delta F P c Q P',
-  semax_ram Delta (Build_SingleFrame P' P nil :: F) P' c Q ->
+  (exists F0: SingleFrame' P' P nil,
+     semax_ram Delta (RAM_FRAME.Build_SingleFrame P' P nil F0 :: F) P' c Q) ->
   semax_ram Delta F P c Q.
 Proof.
   intros.
-  destruct H as [F0 [? [_ ?]]].
+  destruct H as [F0 ?].
+  simpl in H.
+  destruct F0 as [F0 ? ?].  
   eapply semax_ram_pre; eauto.
 Qed.
 
-Lemma semax_ram_unlocalize: forall Delta l g s F P c Q P',
+Lemma semax_ram_unlocalize: forall Delta l g s F P c Q P'
+  (frame_sound: g |-- l * (P -* P'))
+  (frame_closed: Forall (fun s => closed_wrt_modvars s (P -* P')) s),
   semax_ram Delta F P' c Q ->
-  g |-- l * (P -* P') ->
-  Forall (fun s => closed_wrt_modvars s (P -* P')) s ->
-  semax_ram Delta (Build_SingleFrame l g s :: F) P c Q.
+  semax_ram Delta
+   (RAM_FRAME.Build_SingleFrame l g s
+     (RAM_FRAME.Build_SingleFrame' (P -* P') frame_sound frame_closed) :: F) P c Q.
 Proof.
   intros.
-  exists (P -* P').
-  split; [| split]; auto.
+Opaque LiftNatDed' LiftSepLog'.
+  simpl.
+Transparent LiftNatDed' LiftSepLog'.
   eapply semax_ram_pre; [| eauto].
   rewrite sepcon_comm.
   apply wand_sepcon_adjoint.
   auto.
 Qed.
 
-Lemma semax_ram_abduction: forall Delta l g s F P c Q
-  (abd: sigT (fun F0 => g = l * F0)),
-  semax_ram Delta F (P * (projT1 abd)) c Q ->
-  Forall (fun s => closed_wrt_modvars s (projT1 abd)) s ->
-  semax_ram Delta (Build_SingleFrame l g s :: F) P c Q.
+Lemma semax_ram_abduction: forall Delta l g s F P c Q F0
+  (frame_sound: g |-- l * F0)
+  (frame_closed: Forall (fun s => closed_wrt_modvars s F0) s),
+  semax_ram Delta F (P * F0) c Q ->
+  semax_ram Delta
+    (RAM_FRAME.Build_SingleFrame l g s
+      (RAM_FRAME.Build_SingleFrame' F0 frame_sound frame_closed) :: F) P c Q.
 Proof.
   intros.
-  destruct abd as [F0 ?].
-  exists F0.
-  split; [| split]; auto.
-  subst; auto.
+Opaque LiftNatDed' LiftSepLog'.
+  simpl.
+Transparent LiftNatDed' LiftSepLog'.
+  eapply semax_ram_pre; [| eauto]; auto.
 Qed.
 
-Lemma semax_ram_seq: forall Delta F P Q R c0 c1,
+Lemma semax_ram_seq: forall Delta F F' P Q R c0 c1,
+  add_stats c0 F F' ->
   semax Delta P c0 (normal_ret_assert Q) ->
-  semax_ram (update_tycon Delta c0) (add_stats c0 F) Q c1 R ->
+  semax_ram (update_tycon Delta c0) F' Q c1 R ->
   semax_ram Delta F P (Ssequence c0 c1) R.
 Proof.
   intros.
 Opaque LiftNatDed' LiftSepLog'.
-  revert P Q H0 H; induction F; intros; simpl in H0 |- *.
+  revert P Q H0 H1; induction H; intros; simpl in H1 |- *.
 Transparent LiftNatDed' LiftSepLog'.
   + eapply semax_seq'; eauto.
-  + destruct a as [l g s].
-    destruct H0 as [F0 [? [? ?]]].
-    exists F0; split; [| split; [inversion H1 |]]; auto.
-    eapply IHF; [eauto |].
+  + eapply IHadd_stats; [| eauto].
     rewrite <- frame_normal.
     apply semax_frame; auto.
-    inversion H1; subst; auto.
+    inversion fc'; subst; auto.
 Qed.
 
+Lemma ram_seq_assoc: forall Delta F P s1 s2 s3 R,
+  semax_ram Delta F P (Ssequence s1 (Ssequence s2 s3)) R <->
+  semax_ram Delta F P (Ssequence (Ssequence s1 s2) s3) R.
+Proof.
+  induction F; intros.
+  + apply seq_assoc.
+  + simpl.
+    destruct a as [l g s [F0 ? ?]].
+    apply IHF; auto.
+Qed.
+
+Lemma ram_extract_exists_pre: forall A Delta F P c Q,
+  (forall x : A, semax_ram Delta F (P x) c Q) ->
+  semax_ram Delta F (EX  x : A, P x) c Q.
+Proof.
+Opaque LiftNatDed' LiftSepLog'.
+  induction F; intros; simpl in H |- *.
+Transparent LiftNatDed' LiftSepLog'.
+  + apply extract_exists_pre; auto.
+  + destruct a as [l g s [F0 ? ?]].
+    rewrite exp_sepcon1.
+    apply IHF; auto.
+Qed.
+  
 End SEMAX.
