sample_mark/verif_mark.v
@@ -1,22 +1,31 @@
 Require Import RamifyCoq.sample_mark.env_mark.
+Require Import RamifyCoq.graph.graph.
+Require Import RamifyCoq.data_structure.spatial_graph.
+Require Import RamifyCoq.data_structure.spatial_graph_VST.
 
 Local Open Scope logic.
 
-Variable BiMathGraph: Type.
-Variable graph: val -> BiMathGraph -> mpred.
-Variable mark_graph: BiMathGraph -> val -> BiMathGraph.
+Arguments SingleFrame' {l} {g} {s}.
+
+Variable mark: forall {N} {D} {null} {DEC}, @BiMathGraph N D null DEC -> N -> @BiMathGraph N D null DEC -> Prop.
+
+Hypothesis mark_null: forall {N} {D} {null} {DEC} (g g': @BiMathGraph N D null DEC) , mark g null g' -> g = g'.
+
+Definition Graph := @BiMathGraph pointer_val int NullPointer (@AddrDec SGS_VST).
+
+Definition graph sh x (g: Graph): mpred := @graph (SGA_VST sh) x g.
 
 Definition mark_spec :=
  DECLARE _mark
-  WITH g: BiMathGraph, x: val
+  WITH sh: share, g: Graph, g': Graph, x: pointer_val
   PRE [ _x OF (tptr (Tstruct _Node noattr))]
-          PROP  ()
-          LOCAL (temp _x x)
-          SEP   (`(graph x g))
+          PROP  (mark g x g')
+          LOCAL (temp _x (pointer_val_val x))
+          SEP   (`(graph sh x g))
   POST [ tint ]
         PROP ()
         LOCAL()
-        SEP (`(graph x (mark_graph g x))).
+        SEP (`(graph sh x g')).
 
 Definition main_spec :=
  DECLARE _main
@@ -24,6 +33,145 @@ Definition main_spec :=
   PRE  [] main_pre prog u
   POST [ tint ] main_post prog u.
 
-Definition Vprog : varspecs := (_hd, tptr (talignas 4%N (Tstruct _Node noattr)))::(_n, (talignas 4%N (Tstruct _Node noattr)))::nil.
+Definition Vprog : varspecs := (_hd, tptr (Tstruct _Node noattr))::(_n, (Tstruct _Node noattr))::nil.
 
 Definition Gprog : funspecs := mark_spec :: main_spec::nil.
+
+Lemma destruct_pointer_val_VP: forall x,
+  pointer_val_val x <> nullval \/
+  isptr (pointer_val_val x) ->
+  exists b i, x = ValidPointer b i.
+Proof.
+  intros.
+  destruct x; try simpl in H; try tauto.
+  exists b, i; auto.
+Qed.
+
+Lemma destruct_pointer_val_NP: forall x,
+  pointer_val_val x = nullval \/
+  ~ isptr (pointer_val_val x) ->
+  x = NullPointer.
+Proof.
+  intros.
+  destruct x; try simpl in H; try tauto.
+  inversion H; try tauto.
+  inversion H0.
+Qed.
+
+Ltac destruct_pointer_val x :=
+  first [
+    let H := fresh "H" in
+    assert (exists b i, x = ValidPointer b i) by (apply (destruct_pointer_val_VP x); tauto);
+    destruct H as [?b [?i ?H]]
+  | assert (x = NullPointer) by (apply (destruct_pointer_val_NP x); tauto)].
+
+Ltac ram_simplify_Delta :=
+  match goal with
+  | |- semax_ram ?D _ _ _ _ => simplify_Delta_at D
+  | _ => idtac
+  end.
+
+Ltac clear_RamFrame_abbr :=
+  repeat match goal with
+             | H := @abbreviate (list SingleFrame) _ |- _ => 
+                        unfold H, abbreviate; clear H 
+             | H := _: @SingleFrame' _ _ _ |- _ => 
+                        unfold H, abbreviate; clear H 
+            end.
+  
+Ltac abbreviate_RamFrame_rec F RamFrame :=
+  match F with
+  | nil => idtac
+  | RAM_FRAME.Build_SingleFrame ?l ?g ?s ?f :: ?F_tail =>
+      abbreviate_RamFrame_rec F_tail RamFrame;
+      let RamFrame0 := fresh "RamFrame" in
+      set (RamFrame0 := f) in RamFrame;
+      try change @RAM_FRAME.SingleFrame' with @SingleFrame' in RamFrame0
+  end.
+
+Ltac abbreviate_RamFrame :=
+  clear_RamFrame_abbr;
+  match goal with
+  | |- semax_ram _ ?F _ _ _ =>
+         let RamFrame := fresh "RamFrame" in
+         set (RamFrame := @abbreviate (list SingleFrame) F);
+         replace F with RamFrame by reflexivity;
+         abbreviate_RamFrame_rec F RamFrame
+  end.
+
+Ltac abbreviate_semax_ram :=
+  match goal with
+  | |- semax_ram _ _ _ _ _ =>
+         ram_simplify_Delta; unfold_abbrev';
+         match goal with |- semax_ram ?D _ _ ?C ?P => 
+            abbreviate D : tycontext as Delta;
+            abbreviate P : ret_assert as POSTCONDITION ;
+            match C with
+            | Ssequence ?C1 ?C2 =>
+               (* use the next 3 lines instead of "abbreviate"
+                  in case C1 contains an instance of C2 *)
+                let MC := fresh "MORE_COMMANDS" in
+                pose (MC := @abbreviate _ C2);
+                change C with (Ssequence C1 MC);
+                match C1 with
+                | Swhile _ ?C3 => abbreviate C3 as LOOP_BODY
+                | _ => idtac
+                end
+            | Swhile _ ?C3 => abbreviate C3 as LOOP_BODY
+            | _ => idtac
+            end
+        end
+  end;
+  abbreviate_RamFrame;
+  clear_abbrevs;
+  simpl typeof.
+
+Ltac localize P :=
+  match goal with
+  | |- semax ?Delta ?Pre ?c ?Post =>
+         change (semax Delta Pre c Post) with (semax_ram Delta nil Pre c Post);
+         abbreviate_RamFrame
+  end;
+  match goal with
+  | RamFrame := @abbreviate (list SingleFrame) ?F |-
+    semax_ram ?Delta _ ?Pre ?c ?Post =>
+         apply semax_ram_localize with P; eexists;
+         abbreviate_RamFrame
+  end.
+
+Lemma body_mark: semax_body Vprog Gprog f_mark mark_spec.
+Proof.
+  start_function.
+  forward_if_tac  (* if (x == 0) *)
+    (PROP  (pointer_val_val x <> nullval)  LOCAL  (temp _x (pointer_val_val x))  SEP  (`(graph sh x g))); try destruct_pointer_val x.
+  Focus 1. { (* if-then branch *)
+    forward. (* return *)
+    rewrite (mark_null g g') by auto.
+    auto.
+  } Unfocus.
+  Focus 1. { (* if-else branch *)
+    forward. (* skip; *)
+    entailer!.
+  } Unfocus.
+  normalize.
+  destruct_pointer_val x; clear H0.
+
+  remember (gamma (@bm_bi _ _ _ _ g) x) as dlr eqn:?H.
+  destruct dlr as [[d l] r].
+  localize
+   (PROP  ()
+    LOCAL (temp _x (pointer_val_val x))
+    SEP   (`(data_at sh node_type (Vint d, (pointer_val_val l, pointer_val_val r))
+              (pointer_val_val x)))).
+
+  apply -> ram_seq_assoc. 
+  eapply semax_ram_seq;
+    [ repeat apply eexists_add_stats_cons; constructor
+    | new_load_tac 
+    | abbreviate_semax_ram].
+  (* root_mark = x -> m; *)
+  
+  apply ram_extract_exists_pre.
+  intro root_mark_old; autorewrite with subst; clear root_mark_old.
+
+Abort.
